feat: ctxEquiv_of_denoteEquiv

EffectSSA/ProofSketch/ProofSketch.lean
@@ -792,7 +792,7 @@ when for any complete context `C` such that `C[I]` and `C[J]` are both
 wellformed, `C[I]` is (denotationally) equivalent to `C[J]`.
 -/
 def Pattern.CtxEquiv (I J : Pattern n) : Prop :=
-  ∀ (C : MultiContext n),
+  ∀ (C : MultiContext n), C.Complete →
     let CI := C.plug I;
     let CJ := C.plug J;
     CI.WellFormed ∅ → CJ.WellFormed ∅ →
@@ -992,14 +992,14 @@ theorem Pattern.ctxRefine_of_denoteRefine (I J : Pattern n)
         · apply Invariant.of_invariant_cons_hole hI hCI
         · apply Invariant.of_invariant_cons_hole hJ hCJ
 
--- /--
--- Proving denotational equivalence is sufficient for showing contextual equivalence.
--- -/
--- theorem Pattern.ctxEquiv_of_denoteEquiv (I J : Pattern n)
---     (hI : I.HasEqn) (hJ : J.HasEqn) (h_denoteEquiv : I.DenEquiv J) :
---     I.CtxEquiv J := by
---   intro C hC CI CJ ρ
---   have : I.DenRefine J ∧ J.DenRefine I := by grind [DenRefine, DenEquiv]
---   apply SEnv.refine_antisymm
---   <;> apply ctxRefine_of_denoteRefine
---   <;> grind
+/--
+Proving denotational equivalence is sufficient for showing contextual equivalence.
+-/
+theorem Pattern.ctxEquiv_of_denoteEquiv (I J : Pattern n)
+    (hI : I.HasEqn) (hJ : J.HasEqn) (h_denoteEquiv : I.DenEquiv J) :
+    I.CtxEquiv J := by
+  intro C hC CI CJ hCI hCJ
+  have : I.DenRefine J ∧ J.DenRefine I := by grind [DenRefine, DenEquiv]
+  apply SEnv.refine_antisymm
+  <;> apply ctxRefine_of_denoteRefine
+  <;> grind
